{
 "cells": [
  {
   "cell_type": "markdown",
   "metadata": {},
   "source": []
  },
  {
   "cell_type": "markdown",
   "metadata": {},
   "source": [
    "## A\n",
    "\n",
    "**Given system of equations:**\n",
    "\n",
    "1.  $x + y - z = 6$\n",
    "2.  $x + 2y + z = 0$\n",
    "\n",
    "**Step 1: Write the augmented matrix**\n",
    "\n",
    "The augmented matrix represents the system of equations:\n",
    "\n",
    "$\\begin{bmatrix} 1 & 1 & -1 & | & 6 \\\\ 1 & 2 & 1 & | & 0 \\end{bmatrix}$\n",
    "\n",
    "**Step 2: Perform row operations to get the matrix in row-echelon form**\n",
    "\n",
    "We want to get a leading 1 in the first row, first column (which we already have) and zeros below it.  \n",
    "\n",
    "* **R2 = R2 - R1** (Replace row 2 with row 2 minus row 1):\n",
    "\n",
    "$\\begin{bmatrix} 1 & 1 & -1 & | & 6 \\\\ 0 & 1 & 2 & | & -6 \\end{bmatrix}$\n",
    "\n",
    "Now the matrix is in row-echelon form.\n",
    "\n",
    "**Step 3: Convert the matrix back into equations**\n",
    "\n",
    "The matrix represents the following equations:\n",
    "\n",
    "1.  $x + y - z = 6$\n",
    "2.  $y + 2z = -6$\n",
    "\n",
    "**Step 4: Use back substitution to solve for the variables**\n",
    "\n",
    "We have two equations and three unknowns, so we'll solve for x and y in terms of z.\n",
    "\n",
    "From equation (2):\n",
    "\n",
    "* $y = -6 - 2z$\n",
    "\n",
    "Substitute this value of y into equation (1):\n",
    "\n",
    "* $x + (-6 - 2z) - z = 6$\n",
    "* $x - 6 - 2z - z = 6$\n",
    "* $x - 3z = 12$\n",
    "* $x = 12 + 3z$\n",
    "\n",
    "**Solution**\n",
    "\n",
    "The solution to the system is:\n",
    "\n",
    "* $x = 12 + 3z$\n",
    "* $y = -6 - 2z$\n",
    "* $z = z$ (z is a free variable, meaning it can take any value)"
   ]
  },
  {
   "cell_type": "markdown",
   "metadata": {},
   "source": [
    "## B\n",
    "\n",
    "**Given system of equations:**\n",
    "\n",
    "1.  $10x + y = 8$\n",
    "2.  $x + y = 3$\n",
    "\n",
    "**Method: Elimination**\n",
    "\n",
    "* Subtract equation (2) from equation (1):\n",
    "   $(10x + y) - (x + y) = 8 - 3$\n",
    "   $9x = 5$\n",
    "   $x = \\frac{5}{9}$\n",
    "\n",
    "* Substitute $x = \\frac{5}{9}$ into equation (2):\n",
    "   $\\frac{5}{9} + y = 3$\n",
    "   $y = 3 - \\frac{5}{9}$\n",
    "   $y = \\frac{27}{9} - \\frac{5}{9}$\n",
    "   $y = \\frac{22}{9}$\n",
    "\n",
    "**Solution:**\n",
    "\n",
    "$x = \\frac{5}{9}$\n",
    "\n",
    "$y = \\frac{22}{9}$ \n",
    "\n",
    "or \n",
    "\n",
    "$\\left(\\frac{5}{9}, \\frac{22}{9}\\right)$"
   ]
  },
  {
   "cell_type": "markdown",
   "metadata": {},
   "source": [
    "## C\n",
    "**Given system of equations:**\n",
    "\n",
    "1.  $x - y + 4z = -3$\n",
    "2.  $3x + y - z = 8$\n",
    "3.  $x + y + z = 2$\n",
    "\n",
    "**Augmented Matrix:**\n",
    "\n",
    "$\\begin{bmatrix} 1 & -1 & 4 & | & -3 \\\\ 3 & 1 & -1 & | & 8 \\\\ 1 & 1 & 1 & | & 2 \\end{bmatrix}$\n",
    "\n",
    "**Row Operations:**\n",
    "\n",
    "* R2 = R2 - 3R1:  $\\begin{bmatrix} 1 & -1 & 4 & | & -3 \\\\ 0 & 4 & -13 & | & 17 \\\\ 1 & 1 & 1 & | & 2 \\end{bmatrix}$\n",
    "* R3 = R3 - R1: $\\begin{bmatrix} 1 & -1 & 4 & | & -3 \\\\ 0 & 4 & -13 & | & 17 \\\\ 0 & 2 & -3 & | & 5 \\end{bmatrix}$\n",
    "* R3 = 2R3 - R2: $\\begin{bmatrix} 1 & -1 & 4 & | & -3 \\\\ 0 & 4 & -13 & | & 17 \\\\ 0 & 0 & 7 & | & -7 \\end{bmatrix}$\n",
    "\n",
    "**Back Substitution:**\n",
    "\n",
    "* $7z = -7 \\implies z = -1$\n",
    "* $4y - 13(-1) = 17 \\implies y = 1$\n",
    "* $x - 1 + 4(-1) = -3 \\implies x = 2$\n",
    "\n",
    "**Solution:**\n",
    "\n",
    "* $x = 2$\n",
    "* $y = 1$\n",
    "* $z = -1$\n",
    "\n",
    "or $(2, 1, -1)$"
   ]
  }
 ],
 "metadata": {
  "language_info": {
   "name": "python"
  }
 },
 "nbformat": 4,
 "nbformat_minor": 2
}
